ironfleet/src/Dafny/Distributed/Protocol/RSL/FailureProof/Phase2Proof_helper.i.dfy
@@ -1,25 +1,25 @@
-include "Phase2Proof_postFail.i.dfy"
+include "Phase2Proof.i.dfy"
 
 module Rs2Phase2Proof_Helper {
 import opened RslPhase2Proof_postFail_i
 
 
 /* Note: this requires a long timeout to verify */
-lemma PacketsBallotInvariant_ReceiveStep(ts:TimestampedRslState, ts':TimestampedRslState, req_time:Timestamp, opn:OperationNumber, idx:int, tios:seq<TimestampedLIoOp<NodeIdentity, RslMessage>>) 
+lemma PacketsBallotInvariant_ReceiveStep(ts:TimestampedRslState, ts':TimestampedRslState, opn:OperationNumber, idx:int, tios:seq<TimestampedLIoOp<NodeIdentity, RslMessage>>) 
     requires RslAssumption(ts) && RslConsistency(ts)
     requires RslAssumption(ts') && RslConsistency(ts')
     requires TimestampedRslNext(ts, ts')
-    requires RslPerfInvariant(ts, req_time, opn)
+    requires RslPerfInvariant(ts, opn)
     requires TimestampedRslNextOneReplica(ts, ts', idx, tios);
     requires ts.t_replicas[idx].v.nextActionIndex == 0 
     ensures PacketsBallotInvariant(ts')
 {}
 
-lemma PacketsBallotInvariant_NoReceiveStep(ts:TimestampedRslState, ts':TimestampedRslState, req_time:Timestamp, opn:OperationNumber, idx:int, tios:seq<TimestampedLIoOp<NodeIdentity, RslMessage>>) 
+lemma PacketsBallotInvariant_NoReceiveStep(ts:TimestampedRslState, ts':TimestampedRslState, opn:OperationNumber, idx:int, tios:seq<TimestampedLIoOp<NodeIdentity, RslMessage>>) 
     requires RslAssumption(ts) && RslConsistency(ts)
     requires RslAssumption(ts') && RslConsistency(ts')
     requires TimestampedRslNext(ts, ts')
-    requires RslPerfInvariant(ts, req_time, opn)
+    requires RslPerfInvariant(ts, opn)
     requires TimestampedRslNextOneReplica(ts, ts', idx, tios);
     requires ts.t_replicas[idx].v.nextActionIndex != 0 
     ensures PacketsBallotInvariant(ts')
