ironfleet/src/Dafny/Distributed/Protocol/RSL/FailureProof/Phase2Proof_toplevel.i.dfy
@@ -1,5 +1,5 @@
-include "Phase2Proof_postFail.i.dfy"
-include "Phase2Proof_postFail_helper.i.dfy"
+include "Phase2Proof.i.dfy"
+include "Phase2Proof_helper.i.dfy"
 
 module Rs2Phase2Proof_Top {
 import opened RslPhase2Proof_postFail_i
@@ -11,15 +11,17 @@ lemma PerfInvariantMaintained(s:TimestampedRslState, s':TimestampedRslState, req
     requires RslAssumption(s) && RslConsistency(s)
     requires RslAssumption(s') && RslConsistency(s')
     requires TimestampedRslNext(s, s')
-    requires RslPerfInvariant(s, req_time, opn)
-    ensures RslPerfInvariant(s', req_time, opn)
+    requires RslPerfInvariant(s, opn)
+    ensures RslPerfInvariant(s', opn)
 {   
-    PacketsBallotInvariantMaintained(s, s', req_time, opn);
+    PacketsBallotInvariant_Maintained(s, s', opn);
     assert PacketsBallotInvariant(s');
     
+    PerformanceGuarantee_2a_Maintained(s, s', opn);
+    assert PerformanceGuarantee_2a(s', opn);
+    
     assume false;
-    assert PerformanceGuarantee_2a(s');
-    assert PerformanceGuarantee(s');
+    assert PerformanceGuarantee(s', opn);
 }
 
 
@@ -27,11 +29,11 @@ lemma PerfInvariantMaintained(s:TimestampedRslState, s':TimestampedRslState, req
 *                                         Lemmas                                         *
 *****************************************************************************************/
 
-lemma PacketsBallotInvariantMaintained(ts:TimestampedRslState, ts':TimestampedRslState, req_time:Timestamp, opn:OperationNumber) 
+lemma PacketsBallotInvariant_Maintained(ts:TimestampedRslState, ts':TimestampedRslState, opn:OperationNumber) 
     requires RslAssumption(ts) && RslConsistency(ts)
     requires RslAssumption(ts') && RslConsistency(ts')
     requires TimestampedRslNext(ts, ts')
-    requires RslPerfInvariant(ts, req_time, opn)
+    requires RslPerfInvariant(ts, opn)
     ensures PacketsBallotInvariant(ts')
 {
     if TimestampedRslNextEnvironment(ts, ts') {
@@ -41,10 +43,45 @@ lemma PacketsBallotInvariantMaintained(ts:TimestampedRslState, ts':TimestampedRs
     var idx, tios:seq<TimestampedLIoOp<NodeIdentity, RslMessage>> :| TimestampedRslNextOneReplica(ts, ts', idx, tios);
     var nextActionIndex := ts.t_replicas[idx].v.nextActionIndex;
     if nextActionIndex == 0 {
-        PacketsBallotInvariant_ReceiveStep(ts, ts', req_time, opn, idx, tios);
+        PacketsBallotInvariant_ReceiveStep(ts, ts', opn, idx, tios);
     } else {
-        PacketsBallotInvariant_NoReceiveStep(ts, ts', req_time, opn, idx, tios);
+        PacketsBallotInvariant_NoReceiveStep(ts, ts', opn, idx, tios);
     }
+}
+
+lemma PerformanceGuarantee_2a_Maintained(ts:TimestampedRslState, ts':TimestampedRslState, opn:OperationNumber) 
+    requires RslAssumption(ts) && RslConsistency(ts)
+    requires RslAssumption(ts') && RslConsistency(ts')
+    requires PacketsBallotInvariant(ts) && PacketsBallotInvariant(ts')
+    requires TimestampedRslNext(ts, ts')
+    requires RslPerfInvariant(ts, opn)
+    ensures PerformanceGuarantee_2a(ts', opn);
+{
+    if TimestampedRslNextEnvironment(ts, ts') {
+        assert PerformanceGuarantee_2a(ts', opn);
+        return;
+    }
+    if exists pkt :: pkt in ts.t_environment.sentPackets && IsNew2aPacket(pkt, opn) {
+        /* TODO: I can't say anything about leader timestamp at this point.
+        Leader could send new 2a's out. And these 2a's will be unbounded
+        */
+
+        forall pkt | pkt in ts'.undeliveredPackets && IsNew2aPacket(pkt, opn)
+        ensures TimeLe(pkt.msg.ts, TimeBound2aDeliveryPost())
+        {}
+        assert PerformanceGuarantee_2a(ts', opn);
+        return;
+    }
+    
+    var idx, tios:seq<TimestampedLIoOp<NodeIdentity, RslMessage>> :| TimestampedRslNextOneReplica(ts, ts', idx, tios);
+    if idx != 1 {
+        assert PerformanceGuarantee_2a(ts', opn);
+        return;
+    }
+    
+    var nextActionIndex := ts.t_replicas[idx].v.nextActionIndex;
+    assert nextActionIndex == 3;
+    assert PerformanceGuarantee_2a(ts', opn);
 }
 
 }
