ironfleet/src/Dafny/Distributed/Protocol/RSL/FailureProof/verify.sh
@@ -1,7 +1,7 @@
 #!/bin/bash -li
 
-dafnylong Phase2Proof_postFail_helper.i.dfy | grep -iv "Warning"
+dafnylong Phase2Proof_helper.i.dfy | grep -iv "Warning"
 
-dafny Phase2Proof_postFail.i.dfy | grep -iv "Warning"
+dafny Phase2Proof.i.dfy | grep -iv "Warning"
 
 dafny Phase2Proof_toplevel.i.dfy | grep -iv "Warning"
